Prove a few admits

io/Compiler.Model.fst
@@ -180,36 +180,63 @@ let phase1_rrhc () : Lemma (rrhc phase1) by (norm [delta_only [`%rrhc]]) =
 open FStar.List
 
 (** ** Test 1 - FO **)
-let test_interface : iio_interface = {
-  spec_pi = (fun _ _ _ -> true);
-  inst_pi = (fun _ _ _ -> true);
-  inst_pi_stronger_spec_pi = ();
+let ex1_ct_post = (fun () h (rfd:resexn file_descr) lt -> (forall fd'. ~((EOpenfile "/etc/passwd" fd') `List.memP` lt)) /\ (Inl? rfd ==> is_open (Inl?.v rfd) (rev lt @ h)))
+let ex1_spec_pi : monitorable_prop = (fun cmd arg h -> match cmd, arg with | Openfile, s -> if s = "/etc/passwd" then false else true | _ -> true)
+let ex1_inst_pi : monitorable_prop = (fun cmd arg h -> match cmd with | Openfile -> false | _ -> true)
+let ex1_ct_rc = (fun () h (rfd:resexn file_descr) lt -> Inl? rfd && (is_open (Inl?.v rfd) (rev lt @ h)))
 
-  pt = (fun fl -> (unit -> IIO (resexn unit) (fl + IOActions) (fun _ -> True) (fun _ _ _ -> true)));
+let rec ex1_c1post0 (h:trace) (lt:trace) : Lemma
+  (requires (enforced_locally ex1_spec_pi h lt))
+  (ensures (ex1_ct_post () h (Inr Contract_failure) lt))
+  (decreases lt) =
+  match lt with
+  | [] -> ()
+  | e :: tail -> ex1_c1post0 (e::h) tail
 
-  ct = (fun fl -> unit -> IIO (resexn file_descr) fl (fun _ -> True) (fun h rfd lt -> Inl? rfd ==> is_open (Inl?.v rfd) (rev lt @ h)));
-  ct_rcs = Node (| unit, resexn file_descr, (fun () h (rfd:resexn file_descr) lt -> Inl? rfd && (is_open (Inl?.v rfd) (rev lt @ h))) |) Leaf Leaf;
+val ex1_c1post : squash (forall h lt. enforced_locally ex1_spec_pi h lt ==> (ex1_ct_post () h (Inr Contract_failure) lt))
+let ex1_c1post = Classical.forall_intro_2 (Classical.move_requires_2 ex1_c1post0)
+
+val ex1_c2post : squash (forall x h r lt. enforced_locally ex1_spec_pi h lt /\ (ex1_ct_rc x h r lt) ==> ex1_ct_post x h r lt)
+let ex1_c2post = ()
+
+let rec ex1_stronger_pis0 (h:trace) (lt:trace) : Lemma
+  (requires (enforced_locally ex1_inst_pi h lt))
+  (ensures (enforced_locally ex1_spec_pi h lt))
+  (decreases lt) =
+  match lt with
+  | [] -> ()
+  | e :: tail -> ex1_stronger_pis0 (e::h) tail
+                                                  
+val ex1_stronger_pis : squash (forall h lt. enforced_locally ex1_inst_pi h lt ==> enforced_locally ex1_spec_pi h lt)
+let ex1_stronger_pis = Classical.forall_intro_2 (Classical.move_requires_2 ex1_stronger_pis0)
+
+let ex1_interface : iio_interface = {
+  spec_pi = ex1_spec_pi;
+  inst_pi = ex1_inst_pi;
+
+  pt = (fun fl -> (unit -> IIO (resexn unit) (fl + IOActions) (fun _ -> True) (fun _ _ _ -> True)));
+
+  ct = (fun fl -> unit -> IIO (resexn file_descr) fl (fun _ -> True) (ex1_ct_post ()));
+  ct_rcs = Node (| unit, resexn file_descr, ex1_ct_rc |) Leaf Leaf;
 
 
   ct_importable = (fun fl -> 
-    let c1post : unit -> squash (forall h lt. enforced_locally (fun _ _ _ -> true) h lt ==> (exists (rfd:resexn file_descr). Inl? rfd ==> is_open (Inl?.v rfd) (rev lt @ h))) = (fun () ->
- //     assert (forall h lt. enforced_locally (fun _ _ _ -> true) h lt ==> (exists (rfd:resexn file_descr). Inl? rfd ==> is_open (Inl?.v rfd) (rev lt @ h)));
-    admit ()) in
- //   let c2post : squash (forall h (rfd:resexn file_descr) lt. Inl? rfd && (is_open (Inl?.v rfd) (rev lt @ h)) ==> (Inl? rfd ==> is_open (Inl?.v rfd) (rev lt @ h))) = () in
-    safe_importable_arrow_pre_post unit file_descr #_ #_ #fl #exportable_unit #importable_file_descr (fun _ _ -> True) (fun () h rfd lt -> Inl? rfd ==> is_open (Inl?.v rfd) (rev lt @ h)) (c1post ()) ());
+    safe_importable_arrow_pre_post unit file_descr #_ #_ #fl #exportable_unit #importable_file_descr (fun _ _ -> True) ex1_ct_post ex1_c1post ex1_c2post);
+  
+  inst_pi_stronger_spec_pi = ex1_stronger_pis;
 }
 
-val test_prog : prog_iio test_interface
-let test_prog #fl ctx () : IIO (resexn unit) (fl + IOActions) (fun _ -> True) (fun _ _ _ -> True) =
+val ex1_prog : prog_iio ex1_interface
+let ex1_prog #fl ctx () : IIO (resexn unit) (fl + IOActions) (fun _ -> True) (fun _ _ _ -> True) =
   let _ = ctx () in
   Inl ()
 
-val test_ctx : ctx_iio test_interface
-let test_ctx #fl eff_rcs io_acts () : IIO (resexn file_descr) fl (fun _ -> True) (fun h rfd lt -> Inl? rfd ==> is_open (Inl?.v rfd) (rev lt @ h)) = 
+val ex1_ctx : ctx_iio ex1_interface
+let ex1_ctx #fl eff_rcs io_acts () : IIO (resexn file_descr) fl (fun _ -> True) (ex1_ct_post ()) = 
   io_acts Openfile "/etc/passwd"
 
-val test_ctx_t : ctx_ilang (comp_int_iio_ilang test_interface)
-let test_ctx_t #fl io_acts () : IIOpi (resexn file_descr) fl (comp_int_iio_ilang test_interface).spec_pi = 
+val ex1_ctx_t : ctx_ilang (comp_int_iio_ilang ex1_interface)
+let ex1_ctx_t #fl io_acts () : IIOpi (resexn file_descr) fl (comp_int_iio_ilang ex1_interface).spec_pi = 
   io_acts Openfile "/etc/passwd"
 
 
